code/experimental/P256/Hacl.Spec.ECDSA.fst
@@ -266,3 +266,27 @@ let ecdsa_verification publicKey r s mLen input =
    xResult = r
 end end   
 
+
+val ecdsa_signature_nist_compliant: 
+  input: lseq uint8 32 -> 
+  privateKey: lseq uint8 32 -> 
+  k: lseq uint8 32 -> 
+  Tot (tuple3 nat nat bool)
+
+let ecdsa_signature_nist_compliant  input privateKey k = 
+  let basePoint = (0x6B17D1F2E12C4247F8BCE6E563A440F277037D812DEB33A0F4A13945D898C296, 0x4FE342E2FE1A7F9B8EE7EB4A7C0F9E162BCE33576B315ECECBB6406837BF51F5, 1) in
+  let (rxN, ryN, rzN), _ = montgomery_ladder_spec k ((0,0,0), basePoint) in 
+  let (xN, _, _) = _norm (rxN, ryN, rzN) in 
+  let z = nat_from_bytes_le input in 
+  let kFelem = nat_from_bytes_le k in 
+  let privateKey = nat_from_bytes_le privateKey in 
+  let resultR = xN % prime_p256_order in
+  let resultS = 0 in 
+    if resultR = 0 then 
+      resultR, resultS, false
+    else 
+      let resultS = (z + resultR * privateKey) * pow kFelem (prime_p256_order - 2) % prime_p256_order in 
+      if (resultS = 0) then 
+	resultR, resultS, false
+      else 
+	resultR, resultS, true
